FormalSystems.lean
@@ -6,5 +6,6 @@ import FormalSystems.Chomsky.Regular.PowersetConstruction
 
 import FormalSystems.Chomsky.ContextFree.ContextFreeGrammar
 import FormalSystems.Chomsky.ContextFree.ContextFreeDerivation
+import FormalSystems.Chomsky.ContextFree.Theorems
 
 import FormalSystems.Computability.Loop
